LF_diamond.v
@@ -1,0 +1,57 @@
+Require Import LF.
+Require Import Map.
+
+Inductive type0 : Type :=
+| tunit : type0
+| tbool : type0
+| tpair : type0 -> type0 -> type0
+| tsum  : type0 * nat -> type0 * nat -> type0
+| tlist : type0 -> nat -> type0.
+
+Inductive type1 : Type :=
+| tfun : nat -> nat -> list type0 -> type0 -> type1.
+
+Module VarEq <: EQ_TYPE.
+
+  Definition t := nat.
+
+  Definition eq := Nat.eqb.
+
+  Theorem eq_refl : forall x,
+    true = eq x x.
+  Proof.
+    intros. unfold eq. Search (Nat.eqb _ _).
+    apply beq_nat_refl.
+  Qed.
+
+End NatEq.
+
+Module NatMap := Make(NatEq).
+
+(* Definition context := var -> option type0. *)
+Definition context := NatMap.t type0.
+
+Print context.
+Definition context_empty : context := fun _ => None.
+Definition context_add (Gamma : context) (p : var * type0) : context :=
+  fun x => let (y, t) := p in if Nat.eqb x y then Some t else Gamma x.
+Definition context_union (Gamma1 Gamma2 : context) : context :=
+  fun x => match Gamma1 x with
+  | Some t => Some t
+  | None => Gamma2 x
+  end.
+
+
+(* Definition 5.1 *)
+Fixpoint erase0 (t : type0) : LF.type0 :=
+  match t with
+  | tunit => LF.tunit
+  | tbool => LF.tbool
+  | tpair t1 t2 => LF.tpair (erase0 t1) (erase0 t2)
+  | tsum (t1, _) (t2, _) => LF.tsum (erase0 t1) (erase0 t2)
+  | tlist t1 _ => LF.tlist (erase0 t1)
+  end.
+
+Fixpoint erase1 (t : type1) : LF.type1 :=
+  let (_, _, t1s, t2) := t in
+  LF.tfun (Vector.of_list (List.map erase0 t1s)) (erase0 t2).
