ListUtil.v
@@ -1,0 +1,34 @@
+Require Import Coq.Lists.List.
+
+Import ListNotations.
+
+Theorem Forall_app : forall (A : Type) (P : A -> Prop) (xs ys : list A),
+  Forall P xs ->
+  Forall P ys ->
+  Forall P (xs ++ ys).
+Proof.
+  intros A P xs ys H1.
+  generalize dependent ys.
+  induction H1; intros ys H2.
+  - assumption.
+  - simpl.
+    auto using Forall_cons.
+Qed.
+
+Inductive Zip {A B : Type} : list A -> list B -> list (A * B) -> Prop :=
+| Zip_nil : Zip [] [] []
+| Zip_cons : forall x y xs ys zs,
+    Zip xs ys zs -> Zip (x :: xs) (y :: ys) ((x, y) :: zs).
+
+Theorem Zip_app : forall (A B : Type) (xs1 xs2 : list A) (ys1 ys2 : list B)
+  (zs1 zs2 : list (A * B)),
+  Zip xs1 ys1 zs1 ->
+  Zip xs2 ys2 zs2 ->
+  Zip (xs1 ++ xs2) (ys1 ++ ys2) (zs1 ++ zs2).
+Proof.
+  intros A B xs1 xs2 ys1 ys2 zs1 zs2 HZip1.
+  generalize dependent zs2.
+  generalize dependent ys2.
+  generalize dependent xs2.
+  induction HZip1; intros xs2 ys2 zs2 HZip2; simpl; auto using Zip_cons.
+Qed.
